src/high/predicates.v
@@ -79,8 +79,14 @@ Section predicates.
   Definition preds_to_ra (preds : gmap loc (enc_predicate))
     : gmapUR loc (@predicateR Σ) := pred_to_ra <$> preds.
 
-  Definition own_all_preds dq preds :=
-    own predicates_name (●{dq} (preds_to_ra preds) : predicatesR).
+  Definition own_all_preds γ dq preds :=
+    own γ (●{dq} (preds_to_ra preds) : predicatesR).
+
+  Definition own_all_full_preds := own_all_preds full_predicates_name.
+
+  Definition own_all_read_preds := own_all_preds read_predicates_name.
+
+  Definition own_all_pers_preds := own_all_preds pers_predicates_name.
 
   Definition encode_predicate `{Countable ST} (ϕ : predicateO ST)
     : enc_predicateO :=
@@ -90,9 +96,15 @@ Section predicates.
     : unwrapped_predicate :=
     encoded_pred_unwrap (encode_predicate ϕ).
 
-  Definition know_pred `{Countable ST} ℓ (ϕ : predicateO ST) : iProp Σ :=
-    own predicates_name
+  Definition know_pred `{Countable ST} γ ℓ (ϕ : predicateO ST) : iProp Σ :=
+    own γ
         (◯ {[ ℓ := unwrapped_pred_to_ra (predicate_to_unwrapped_predicate ϕ) ]}).
+
+  Definition know_full_pred `{Countable ST} := know_pred (ST := ST) full_predicates_name.
+
+  Definition know_read_pred `{Countable ST} := know_pred (ST := ST) read_predicates_name.
+
+  Definition know_pers_pred `{Countable ST} := know_pred (ST := ST) pers_predicates_name.
 
   Local Instance unwrapped_pred_to_ra_contractive :
     Contractive unwrapped_pred_to_ra.
@@ -123,8 +135,8 @@ Section predicates.
     apply (H0 _ _).
   Qed.
 
-  Global Instance know_pred_contractive `{Countable ST} ℓ :
-    Contractive (know_pred (ST := ST) ℓ).
+  Lemma know_pred_contractive `{Countable ST} γ ℓ:
+    Contractive (know_pred (ST := ST) γ ℓ).
   Proof.
     intros ????.
     rewrite /know_pred.
@@ -135,6 +147,15 @@ Section predicates.
     rewrite H0.
     f_equiv.
   Qed.
+
+  Global Instance know_full_pred_contractive `{Countable ST} ℓ :
+    Contractive (know_full_pred (ST := ST) ℓ) := know_pred_contractive (ST := ST) full_predicates_name ℓ.
+
+  Global Instance know_read_pred_contractive `{Countable ST} ℓ :
+    Contractive (know_read_pred (ST := ST) ℓ) := know_pred_contractive (ST := ST) read_predicates_name ℓ.
+
+  Global Instance know_pers_pred_contractive `{Countable ST} ℓ :
+    Contractive (know_pers_pred (ST := ST) ℓ) := know_pred_contractive (ST := ST) pers_predicates_name ℓ.
 
   Lemma encode_predicate_extract `{Countable ST}
       (ϕ : predicate ST) e s v
@@ -189,10 +210,10 @@ Section predicates.
     iApply "eq".
   Qed.
 
-  Lemma own_all_preds_pred `{Countable ST}
+  Lemma own_all_preds_pred `{Countable ST} γ
         dq ℓ (ϕ : predicate ST) (preds : gmap loc enc_predicate) :
-    own_all_preds dq preds -∗
-    know_pred ℓ ϕ -∗
+    own_all_preds γ dq preds -∗
+    know_pred γ ℓ ϕ -∗
     (∃ (o : enc_predicateO),
        ⌜preds !! ℓ = Some o⌝ ∗ (* Some encoded predicate exists. *)
        ▷ (o ≡ encode_predicate ϕ)).
@@ -241,6 +262,33 @@ Section predicates.
       done.
   Qed.
 
+  Lemma own_all_full_preds_pred `{Countable ST}
+        dq ℓ (ϕ : predicate ST) (preds : gmap loc enc_predicate) :
+    own_all_full_preds dq preds -∗
+    know_full_pred ℓ ϕ -∗
+    (∃ (o : enc_predicateO),
+       ⌜preds !! ℓ = Some o⌝ ∗ (* Some encoded predicate exists. *)
+       ▷ (o ≡ encode_predicate ϕ)).
+    Proof. apply own_all_preds_pred. Qed.
+
+  Lemma own_all_read_preds_pred `{Countable ST}
+        dq ℓ (ϕ : predicate ST) (preds : gmap loc enc_predicate) :
+    own_all_read_preds dq preds -∗
+    know_read_pred ℓ ϕ -∗
+    (∃ (o : enc_predicateO),
+       ⌜preds !! ℓ = Some o⌝ ∗ (* Some encoded predicate exists. *)
+       ▷ (o ≡ encode_predicate ϕ)).
+  Proof. apply own_all_preds_pred. Qed.
+
+  Lemma own_all_pers_preds_pred `{Countable ST}
+        dq ℓ (ϕ : predicate ST) (preds : gmap loc enc_predicate) :
+    own_all_pers_preds dq preds -∗
+    know_pers_pred ℓ ϕ -∗
+    (∃ (o : enc_predicateO),
+       ⌜preds !! ℓ = Some o⌝ ∗ (* Some encoded predicate exists. *)
+       ▷ (o ≡ encode_predicate ϕ)).
+  Proof. apply own_all_preds_pred. Qed.
+
   Lemma predicates_frag_lookup γ predicates (ℓ : loc) pred :
     predicates !! ℓ = Some pred →
     own γ (◯ (pred_to_ra <$> predicates) : predicatesR) -∗
@@ -270,11 +318,11 @@ Section predicates.
     done.
   Qed.
 
-  Lemma own_all_preds_insert `{Countable ST} preds ℓ (ϕ : ST → val → dProp Σ) :
+  Lemma own_all_preds_insert `{Countable ST} γ preds ℓ (ϕ : ST → val → dProp Σ) :
     preds !! ℓ = None →
-    own predicates_name (● preds_to_ra preds) ==∗
-    own predicates_name (● preds_to_ra (<[ℓ := encode_predicate ϕ]>preds)) ∗
-    know_pred ℓ ϕ.
+    own γ (● preds_to_ra preds) ==∗
+    own γ (● preds_to_ra (<[ℓ := encode_predicate ϕ]>preds)) ∗
+    know_pred γ ℓ ϕ.
   Proof.
     iIntros (look) "A".
     rewrite /know_pred.
@@ -288,6 +336,27 @@ Section predicates.
     rewrite fmap_insert.
     iFrame.
   Qed.
+
+  Lemma own_all_full_preds_insert `{Countable ST} full_predicates_name preds ℓ (ϕ : ST → val → dProp Σ) :
+    preds !! ℓ = None →
+    own full_predicates_name (● preds_to_ra preds) ==∗
+    own full_predicates_name (● preds_to_ra (<[ℓ := encode_predicate ϕ]>preds)) ∗
+    know_pred full_predicates_name ℓ ϕ.
+  Proof. apply own_all_preds_insert. Qed.
+
+  Lemma own_all_read_preds_insert `{Countable ST} read_predicates_name preds ℓ (ϕ : ST → val → dProp Σ) :
+    preds !! ℓ = None →
+    own read_predicates_name (● preds_to_ra preds) ==∗
+    own read_predicates_name (● preds_to_ra (<[ℓ := encode_predicate ϕ]>preds)) ∗
+    know_pred read_predicates_name ℓ ϕ.
+  Proof. apply own_all_preds_insert. Qed.
+
+  Lemma own_all_pers_preds_insert `{Countable ST} pers_predicates_name preds ℓ (ϕ : ST → val → dProp Σ) :
+    preds !! ℓ = None →
+    own pers_predicates_name (● preds_to_ra preds) ==∗
+    own pers_predicates_name (● preds_to_ra (<[ℓ := encode_predicate ϕ]>preds)) ∗
+    know_pred pers_predicates_name ℓ ϕ.
+  Proof. apply own_all_preds_insert. Qed.
 
 End predicates.
 
