src/high/locations.v
@@ -188,15 +188,19 @@ Section mapsto_at_lemmas.
     FlushFree (mapsto_at ℓ prot ss).
   Proof. apply _. Qed.
 
-  Global Instance mapsto_at_contractive ℓ ss bumper :
-    Contractive (λ (inv : loc_predO ST), (ℓ ↦_AT^{MkProt inv bumper} ss)).
+  Global Instance mapsto_at_contractive ℓ ss bumper:
+    Contractive (λ (invs : loc_predO ST * loc_predO ST * loc_predO ST),
+                   let '(full, read, pers) := invs in
+                   (ℓ ↦_AT^{MkProt full read pers bumper} ss)).
   Proof.
     rewrite /mapsto_at.
     intros ????.
+    destruct x as [[full read] pers].
+    destruct y as [[full' read'] pers'].
     f_equiv. f_equiv. f_equiv. f_equiv. f_equiv. f_equiv. f_equiv. f_equiv.
     f_equiv. f_equiv. f_equiv. f_equiv. f_equiv. f_equiv. f_equiv. f_equiv.
     f_equiv. f_equiv. f_equiv. f_equiv. f_equiv. f_equiv.
-    apply know_protocol_contractive.
+    apply (know_protocol_contractive ℓ bumper n (ST := ST) (full, read, pers) (full', read', pers')).
     assumption.
   Qed.
 
@@ -792,7 +796,7 @@ Section mapsto_at_lemmas.
     rewrite /mapsto_at.
     iNamed 1.
     iDestruct (know_protocol_extract with "locationProtocol")
-      as "(pred & knowPreorder & knowBumper)".
+      as "(fullPred & readPred & PersPred & knowPreorder & knowBumper)".
     iAssert (□ ∀ t s, know_frag_history_loc_d ℓ t s -∗ _)%I as "#impl".
     { iIntros "!>" (??).
       iApply (post_crash_frag_history with "knowPreorder offset knowBumper"). }
@@ -801,7 +805,7 @@ Section mapsto_at_lemmas.
       iApply "impl". }
     iCrashIntro.
     iDestruct (if_rec_is_persisted ℓ) as "persisted".
-    (* TODO: Why is this [IntoIfRec] instance not picked up automatically. *)
+    (* TODO: Why is this [IntoIfRec] instsance not picked up automatically. *)
     iDestruct (into_if_rec with "HI") as "HH".
     { apply big_sepM_into_if_rec. intros. apply into_if_rec_if_rec. }
     iModIntro.
@@ -874,7 +878,7 @@ Section mapsto_at_lemmas.
     rewrite /mapsto_at.
     iNamed 1.
     iDestruct (know_protocol_extract with "locationProtocol")
-      as "(pred & order & bumper)".
+      as "(FullPred & ReadPred & PersPred & order & bumper)".
     iAssert (□ ∀ t s, know_frag_history_loc_d ℓ t s -∗ _)%I as "#impl".
     { iIntros "!>" (??).
       iApply (post_crash_frag_history with "order offset bumper"). }
